move EqualityType stuff into ml_repl_moduleTheory
the idea is that ml_repl_moduleTheory produces a theorem about the
module that is actually useful, i.e. without all the unnecessary
assumptions. side-bonus: can also define INPUT_TYPE and OUTPUT_TYPE at
this stage, and simplify the theorem with them.

also, put some comments in bootstrap_lemmasScript.sml about other things
that might deserve to be moved elsewhere.

translator/repl/ml_repl_moduleScript.sml
@@ -1,4 +1,4 @@
-open preamble;
+open preamble miscLib;
 open inferTheory inferSoundTheory inferPropsTheory unifyTheory ml_repl_stepTheory;
 open ml_translatorTheory sideTheory;
 
@@ -56,10 +56,577 @@ val module_thm = let
   val thms = th |> Q.SPEC `NONE` |> CONJUNCTS
   in CONJ (hd thms) (last thms) end;
 
-val _ = save_thm("module_thm", module_thm);
+local
+  val ths = ml_translatorLib.eq_lemmas();
+in
+  fun find_equality_type_thm tm =
+    first (can (C match_term tm) o rand o snd o strip_imp o concl) ths
+end
 
-val _ = save_thm("equality_types",
-  LIST_CONJ (ml_translatorLib.eq_lemmas()));
+val EqualityType_thm = prove(
+  ``EqualityType abs ⇔
+      (!x1 v1. abs x1 v1 ==> no_closures v1) /\
+      (!x1 v1 x2 v2. abs x1 v1 /\ abs x2 v2 ==> types_match v1 v2 /\
+                                                ((v1 = v2) ⇔ (x1 = x2)))``,
+  SIMP_TAC std_ss [EqualityType_def] \\ METIS_TAC []);
+val EqualityType_CHAR = find_equality_type_thm``CHAR``
+val EqualityType_INT = find_equality_type_thm``INT``
+val EqualityType_NUM = find_equality_type_thm``NUM``
+val EqualityType_BOOL = find_equality_type_thm``BOOL``
+val EqualityType_WORD8 = find_equality_type_thm``WORD8``
+val EqualityType_SUM_TYPE = find_equality_type_thm``SUM_TYPE a b``
+val EqualityType_LIST_TYPE_CHAR = find_equality_type_thm``LIST_TYPE CHAR``
+  |> Q.GEN`a` |> Q.ISPEC`CHAR` |> SIMP_RULE std_ss [EqualityType_CHAR]
+val EqualityType_TOKENS_TOKEN_TYPE = find_equality_type_thm``TOKENS_TOKEN_TYPE``
+  |> SIMP_RULE std_ss [EqualityType_LIST_TYPE_CHAR,EqualityType_INT,EqualityType_NUM]
+val EqualityType_GRAM_MMLNONT_TYPE = find_equality_type_thm``GRAM_MMLNONT_TYPE``
+  |> SIMP_RULE std_ss []
+val EqualityType_AST_ID_TYPE_LIST_TYPE_CHAR = find_equality_type_thm``AST_ID_TYPE a``
+  |> Q.GEN`a` |> Q.ISPEC`LIST_TYPE CHAR` |> SIMP_RULE std_ss [EqualityType_LIST_TYPE_CHAR]
+val EqualityType_OPTION_TYPE_AST_ID_TYPE_LIST_TYPE_CHAR = find_equality_type_thm``OPTION_TYPE a``
+  |> Q.GEN`a` |> Q.ISPEC`AST_ID_TYPE (LIST_TYPE CHAR)` |> SIMP_RULE std_ss [EqualityType_AST_ID_TYPE_LIST_TYPE_CHAR]
+val EqualityType_AST_LIT_TYPE = find_equality_type_thm``AST_LIT_TYPE``
+  |> SIMP_RULE std_ss [EqualityType_LIST_TYPE_CHAR,EqualityType_INT,EqualityType_BOOL,EqualityType_WORD8]
+val EqualityType_AST_OPN_TYPE = find_equality_type_thm``AST_OPN_TYPE`` |> SIMP_RULE std_ss []
+val EqualityType_AST_OPB_TYPE = find_equality_type_thm``AST_OPB_TYPE`` |> SIMP_RULE std_ss []
+val EqualityType_AST_OP_TYPE = find_equality_type_thm``AST_OP_TYPE``
+  |> SIMP_RULE std_ss [EqualityType_AST_OPB_TYPE,EqualityType_AST_OPN_TYPE]
+val EqualityType_CONLANG_OP_I2_TYPE = find_equality_type_thm``CONLANG_OP_I2_TYPE``
+  |> SIMP_RULE std_ss [EqualityType_NUM,EqualityType_AST_OP_TYPE]
+val EqualityType_PATLANG_OP_PAT_TYPE = find_equality_type_thm``PATLANG_OP_PAT_TYPE``
+  |> SIMP_RULE std_ss [EqualityType_NUM,EqualityType_CONLANG_OP_I2_TYPE]
+val EqualityType_OPTION_TYPE_LIST_TYPE_CHAR = find_equality_type_thm``OPTION_TYPE a``
+  |> Q.GEN`a` |> Q.ISPEC`LIST_TYPE CHAR` |> SIMP_RULE std_ss [EqualityType_LIST_TYPE_CHAR]
+val EqualityType_AST_LOP_TYPE = find_equality_type_thm``AST_LOP_TYPE``
+  |> SIMP_RULE std_ss []
+val EqualityType_PAIR_TYPE = find_equality_type_thm``PAIR_TYPE a b``
+val EqualityType_OPTION_TYPE = (find_equality_type_thm``OPTION_TYPE a``)
+val EqualityType_SEMANTICPRIMITIVES_TID_OR_EXN_TYPE = find_equality_type_thm``SEMANTICPRIMITIVES_TID_OR_EXN_TYPE``
+  |> SIMP_RULE std_ss [EqualityType_AST_ID_TYPE_LIST_TYPE_CHAR]
+val EqualityType_SPTREE_SPT_TYPE_UNIT_TYPE = find_equality_type_thm``SPTREE_SPT_TYPE a``
+  |> Q.GEN`a` |> Q.ISPEC`UNIT_TYPE` |> SIMP_RULE std_ss [find_equality_type_thm``UNIT_TYPE``]
+val EqualityType_LIST_TYPE = find_equality_type_thm``LIST_TYPE a``
+val EqualityType_GRAMMAR_SYMBOL_TYPE = prove(
+  ``∀a b. EqualityType a ∧ EqualityType b ⇒ EqualityType (GRAMMAR_SYMBOL_TYPE a b)``,
+  rw[EqualityType_thm] >- (
+    Cases_on`x1`>>fs[ml_repl_stepTheory.GRAMMAR_SYMBOL_TYPE_def]>>rw[]>>
+    rw[no_closures_def] >- METIS_TAC[] >>
+    METIS_TAC[EqualityType_SUM_TYPE,EqualityType_NUM,EqualityType_thm] )
+  >- (
+    Cases_on`x1`>>Cases_on`x2`>>fs[ml_repl_stepTheory.GRAMMAR_SYMBOL_TYPE_def]>>
+    rw[types_match_def] >- METIS_TAC[] >>
+    METIS_TAC[EqualityType_SUM_TYPE,EqualityType_NUM,EqualityType_thm] )
+  >- (
+    Cases_on`x1`>>Cases_on`x2`>>fs[ml_repl_stepTheory.GRAMMAR_SYMBOL_TYPE_def]>>
+    rw[] >>
+    METIS_TAC[EqualityType_SUM_TYPE,EqualityType_NUM,EqualityType_thm] ))
+
+val _ = temp_tight_equality();
+
+val GRAMMAR_PARSETREE_TYPE_no_closures = prove(
+  ``∀a b c d. EqualityType a ∧ EqualityType b ∧ GRAMMAR_PARSETREE_TYPE a b c d ⇒ no_closures d``,
+  ho_match_mp_tac ml_repl_stepTheory.GRAMMAR_PARSETREE_TYPE_ind >>
+  simp[ml_repl_stepTheory.GRAMMAR_PARSETREE_TYPE_def,PULL_EXISTS,no_closures_def] >>
+  rw[] >- METIS_TAC[EqualityType_SUM_TYPE,EqualityType_NUM,EqualityType_thm]
+  >- (
+    pop_assum mp_tac >>
+    Q.ID_SPEC_TAC`v2_2` >>
+    Induct_on`x_2` >> simp[ml_repl_stepTheory.LIST_TYPE_def,no_closures_def,PULL_EXISTS] >>
+    rw[] >> METIS_TAC[]) >>
+  METIS_TAC[EqualityType_GRAMMAR_SYMBOL_TYPE,EqualityType_thm])
+
+val GRAMMAR_PARSETREE_TYPE_types_match = prove(
+  ``∀a b c d e f.
+      EqualityType a ∧ EqualityType b ∧ GRAMMAR_PARSETREE_TYPE a b c d ∧
+      GRAMMAR_PARSETREE_TYPE a b e f ⇒ types_match d f``,
+  ho_match_mp_tac ml_repl_stepTheory.GRAMMAR_PARSETREE_TYPE_ind >>
+  simp[ml_repl_stepTheory.GRAMMAR_PARSETREE_TYPE_def,PULL_EXISTS,types_match_def] >>
+  rw[] >- (
+    Cases_on`e`>>fs[ml_repl_stepTheory.GRAMMAR_PARSETREE_TYPE_def,types_match_def] >>
+    conj_tac >- METIS_TAC[EqualityType_SUM_TYPE,EqualityType_NUM,EqualityType_thm] >>
+    rw[] >> rpt(rator_x_assum`LIST_TYPE`mp_tac) >>
+    last_x_assum mp_tac >>
+    map_every qid_spec_tac[`v2_2`,`v2_2'`,`x_2`,`l`] >>
+    Induct >> simp[ml_repl_stepTheory.LIST_TYPE_def,PULL_EXISTS] >> rw[] >>
+    Cases_on`x_2`>>fs[ml_repl_stepTheory.LIST_TYPE_def,types_match_def] >>
+    METIS_TAC[]) >>
+  Cases_on`e`>>fs[ml_repl_stepTheory.GRAMMAR_PARSETREE_TYPE_def,types_match_def] >>
+  METIS_TAC[EqualityType_GRAMMAR_SYMBOL_TYPE,EqualityType_thm])
+
+val GRAMMAR_PARSETREE_TYPE_11 = prove(
+  ``∀a b c d e f.
+      EqualityType a ∧ EqualityType b ∧ GRAMMAR_PARSETREE_TYPE a b c d ∧
+      GRAMMAR_PARSETREE_TYPE a b e f ⇒ (c = e ⇔ d = f)``,
+  ho_match_mp_tac ml_repl_stepTheory.GRAMMAR_PARSETREE_TYPE_ind >>
+  simp[ml_repl_stepTheory.GRAMMAR_PARSETREE_TYPE_def,PULL_EXISTS] >>
+  rw[] >- (
+    Cases_on`e`>>fs[ml_repl_stepTheory.GRAMMAR_PARSETREE_TYPE_def] >>
+    `x_3 = s ⇔ v2_1 = v2_1'` by METIS_TAC[EqualityType_SUM_TYPE,EqualityType_NUM,EqualityType_thm] >>
+    rw[] >> rpt(rator_x_assum`LIST_TYPE`mp_tac) >>
+    last_x_assum mp_tac >>
+    map_every qid_spec_tac[`v2_2`,`v2_2'`,`x_2`,`l`] >>
+    Induct >> simp[ml_repl_stepTheory.LIST_TYPE_def,PULL_EXISTS] >> rw[] >>
+    Cases_on`x_2`>>fs[ml_repl_stepTheory.LIST_TYPE_def] >>
+    METIS_TAC[]) >>
+  Cases_on`e`>>fs[ml_repl_stepTheory.GRAMMAR_PARSETREE_TYPE_def] >>
+  METIS_TAC[EqualityType_GRAMMAR_SYMBOL_TYPE,EqualityType_thm])
+
+val EqualityType1 = prove(
+  ``EqualityType (GRAMMAR_PARSETREE_TYPE TOKENS_TOKEN_TYPE GRAM_MMLNONT_TYPE)``,
+  simp[EqualityType_thm] >>
+  assume_tac EqualityType_TOKENS_TOKEN_TYPE >>
+  assume_tac EqualityType_GRAM_MMLNONT_TYPE >>
+  conj_tac >- METIS_TAC[GRAMMAR_PARSETREE_TYPE_no_closures] >>
+  METIS_TAC[GRAMMAR_PARSETREE_TYPE_types_match,GRAMMAR_PARSETREE_TYPE_11])
+
+val EqualityType_AST_TCTOR_TYPE = prove(
+  ``EqualityType AST_TCTOR_TYPE``,
+  rw[EqualityType_thm] >- (
+    Cases_on`x1`>>fs[ml_repl_stepTheory.AST_TCTOR_TYPE_def,no_closures_def] >>
+    METIS_TAC[EqualityType_AST_ID_TYPE_LIST_TYPE_CHAR,EqualityType_thm] )
+  >- (
+    Cases_on`x1`>>Cases_on`x2`>>fs[ml_repl_stepTheory.AST_TCTOR_TYPE_def,types_match_def]>>rw[]>>
+    METIS_TAC[EqualityType_AST_ID_TYPE_LIST_TYPE_CHAR,EqualityType_thm])
+  >- (
+    Cases_on`x1`>>Cases_on`x2`>>fs[ml_repl_stepTheory.AST_TCTOR_TYPE_def]>>rw[]>>
+    METIS_TAC[EqualityType_AST_ID_TYPE_LIST_TYPE_CHAR,EqualityType_thm]))
+
+val AST_T_TYPE_no_closures = prove(
+  ``∀a b. AST_T_TYPE a b ⇒ no_closures b``,
+  ho_match_mp_tac ml_repl_stepTheory.AST_T_TYPE_ind >>
+  simp[ml_repl_stepTheory.AST_T_TYPE_def,PULL_EXISTS,no_closures_def] >> rw[] >- (
+    pop_assum kall_tac >>
+    pop_assum mp_tac >>
+    pop_assum mp_tac >>
+    map_every qid_spec_tac[`v3_1`,`x_4`] >>
+    Induct >> simp[ml_repl_stepTheory.LIST_TYPE_def,no_closures_def,PULL_EXISTS] >>
+    rw[] >> METIS_TAC[] ) >>
+  METIS_TAC[EqualityType_AST_TCTOR_TYPE,EqualityType_thm,EqualityType_NUM,EqualityType_LIST_TYPE_CHAR])
+
+val AST_T_TYPE_types_match = prove(
+  ``∀a b c d. AST_T_TYPE a b ∧ AST_T_TYPE c d ⇒ types_match b d``,
+  ho_match_mp_tac ml_repl_stepTheory.AST_T_TYPE_ind >>
+  simp[ml_repl_stepTheory.AST_T_TYPE_def,PULL_EXISTS,types_match_def] >> rw[] >- (
+    Cases_on`c`>>fs[ml_repl_stepTheory.AST_T_TYPE_def,types_match_def] >>
+    reverse conj_tac >- METIS_TAC[EqualityType_AST_TCTOR_TYPE,EqualityType_thm] >> rw[] >>
+    pop_assum kall_tac >>
+    rator_x_assum`AST_TCTOR_TYPE`kall_tac >>
+    rpt (pop_assum mp_tac) >>
+    map_every qid_spec_tac[`v3_1'`,`v3_1`,`l`,`x_4`] >>
+    Induct >> simp[ml_repl_stepTheory.LIST_TYPE_def,PULL_EXISTS] >- (
+      Cases >> simp[ml_repl_stepTheory.LIST_TYPE_def,types_match_def,PULL_EXISTS] ) >>
+    rw[] >> Cases_on`l`>>fs[ml_repl_stepTheory.LIST_TYPE_def,types_match_def] >>
+    METIS_TAC[] )
+  >- (
+    Cases_on`c`>>fs[ml_repl_stepTheory.AST_T_TYPE_def,types_match_def] >>
+    METIS_TAC[EqualityType_NUM,EqualityType_thm] )
+  >- (
+    Cases_on`c`>>fs[ml_repl_stepTheory.AST_T_TYPE_def,types_match_def] >>
+    METIS_TAC[EqualityType_LIST_TYPE_CHAR,EqualityType_thm] ))
+
+val AST_T_TYPE_11 = prove(
+  ``∀a b c d. AST_T_TYPE a b ∧ AST_T_TYPE c d ⇒ (a = c ⇔ b = d)``,
+  ho_match_mp_tac ml_repl_stepTheory.AST_T_TYPE_ind >>
+  simp[ml_repl_stepTheory.AST_T_TYPE_def,PULL_EXISTS] >> rw[] >- (
+    Cases_on`c`>>fs[ml_repl_stepTheory.AST_T_TYPE_def] >>
+    `x_3 = t ⇔ v3_2 = v3_2'` by METIS_TAC[EqualityType_AST_TCTOR_TYPE,EqualityType_thm] >> rw[] >>
+    rpt(rator_x_assum`AST_TCTOR_TYPE`kall_tac) >>
+    pop_assum kall_tac >>
+    rpt (pop_assum mp_tac) >>
+    map_every qid_spec_tac[`v3_1'`,`v3_1`,`l`,`x_4`] >>
+    Induct >> simp[ml_repl_stepTheory.LIST_TYPE_def,PULL_EXISTS] >- (
+      Cases >> simp[ml_repl_stepTheory.LIST_TYPE_def,PULL_EXISTS] ) >>
+    rw[] >> Cases_on`l`>>fs[ml_repl_stepTheory.LIST_TYPE_def] >>
+    METIS_TAC[] )
+  >- (
+    Cases_on`c`>>fs[ml_repl_stepTheory.AST_T_TYPE_def] >>
+    METIS_TAC[EqualityType_NUM,EqualityType_thm] )
+  >- (
+    Cases_on`c`>>fs[ml_repl_stepTheory.AST_T_TYPE_def] >>
+    METIS_TAC[EqualityType_LIST_TYPE_CHAR,EqualityType_thm] ))
+
+val EqualityType2 = prove(
+  ``EqualityType AST_T_TYPE``,
+  simp[EqualityType_thm] >>
+  METIS_TAC[AST_T_TYPE_no_closures,AST_T_TYPE_types_match,AST_T_TYPE_11])
+
+val AST_PAT_TYPE_no_closures = prove(
+  ``∀a b. AST_PAT_TYPE a b ⇒ no_closures b``,
+  ho_match_mp_tac ml_repl_stepTheory.AST_PAT_TYPE_ind >>
+  simp[ml_repl_stepTheory.AST_PAT_TYPE_def,PULL_EXISTS,no_closures_def] >>
+  rw[] >>
+  TRY (
+    pop_assum mp_tac >>
+    pop_assum kall_tac >>
+    pop_assum mp_tac >>
+    map_every qid_spec_tac[`v3_2`,`x_3`] >>
+    Induct >> simp[ml_repl_stepTheory.LIST_TYPE_def,no_closures_def,PULL_EXISTS] >>
+    rw[] >> METIS_TAC[] ) >>
+  METIS_TAC[EqualityType_thm,
+            EqualityType_OPTION_TYPE_AST_ID_TYPE_LIST_TYPE_CHAR,
+            EqualityType_AST_LIT_TYPE,
+            EqualityType_LIST_TYPE_CHAR])
+
+val AST_PAT_TYPE_types_match = prove(
+  ``∀a b c d. AST_PAT_TYPE a b ∧ AST_PAT_TYPE c d ⇒ types_match b d``,
+  ho_match_mp_tac ml_repl_stepTheory.AST_PAT_TYPE_ind >>
+  simp[ml_repl_stepTheory.AST_PAT_TYPE_def,PULL_EXISTS,types_match_def] >> rw[] >>
+  Cases_on`c`>>fs[ml_repl_stepTheory.AST_PAT_TYPE_def,types_match_def] >> rw[] >>
+  TRY (
+    rpt(rator_x_assum`LIST_TYPE`mp_tac) >>
+    ntac 2 (pop_assum kall_tac) >> pop_assum mp_tac >>
+    map_every qid_spec_tac[`v3_2`,`v3_2'`,`l`,`x_3`] >>
+    Induct >> simp[ml_repl_stepTheory.LIST_TYPE_def] >- (
+      Cases >> simp[ml_repl_stepTheory.LIST_TYPE_def,types_match_def,PULL_EXISTS] ) >>
+    gen_tac >> Cases >> rw[ml_repl_stepTheory.LIST_TYPE_def] >> rw[types_match_def] >>
+    METIS_TAC[] ) >>
+  METIS_TAC[EqualityType_thm,EqualityType_LIST_TYPE_CHAR,EqualityType_AST_LIT_TYPE,
+            EqualityType_OPTION_TYPE_AST_ID_TYPE_LIST_TYPE_CHAR])
+
+val AST_PAT_TYPE_11 = prove(
+  ``∀a b c d. AST_PAT_TYPE a b ∧ AST_PAT_TYPE c d ⇒ (a = c ⇔ b = d)``,
+  ho_match_mp_tac ml_repl_stepTheory.AST_PAT_TYPE_ind >>
+  simp[ml_repl_stepTheory.AST_PAT_TYPE_def,PULL_EXISTS] >> rw[] >>
+  Cases_on`c`>>fs[ml_repl_stepTheory.AST_PAT_TYPE_def] >> rw[] >>
+  TRY (
+    rpt(rator_x_assum`LIST_TYPE`mp_tac) >>
+    `x_4 = o' ⇔ v3_1 = v3_1'` by METIS_TAC[EqualityType_thm,EqualityType_OPTION_TYPE_AST_ID_TYPE_LIST_TYPE_CHAR] >>
+    simp[] >>
+    ntac 3 (pop_assum kall_tac) >> pop_assum mp_tac >>
+    map_every qid_spec_tac[`v3_2`,`v3_2'`,`l`,`x_3`] >>
+    Induct >> simp[ml_repl_stepTheory.LIST_TYPE_def] >- (
+      Cases >> simp[ml_repl_stepTheory.LIST_TYPE_def,PULL_EXISTS] ) >>
+    gen_tac >> Cases >> rw[ml_repl_stepTheory.LIST_TYPE_def] >> rw[] >>
+    METIS_TAC[] ) >>
+  METIS_TAC[EqualityType_thm,EqualityType_LIST_TYPE_CHAR,EqualityType_AST_LIT_TYPE,
+            EqualityType_OPTION_TYPE_AST_ID_TYPE_LIST_TYPE_CHAR])
+
+val EqualityType3 = prove(
+  ``EqualityType AST_PAT_TYPE``,
+  METIS_TAC[EqualityType_thm,AST_PAT_TYPE_no_closures,AST_PAT_TYPE_types_match,AST_PAT_TYPE_11])
+
+val PATLANG_EXP_PAT_TYPE_no_closures = prove(
+  ``∀a b. PATLANG_EXP_PAT_TYPE a b ⇒ no_closures b``,
+  ho_match_mp_tac ml_repl_stepTheory.PATLANG_EXP_PAT_TYPE_ind >>
+  simp[ml_repl_stepTheory.PATLANG_EXP_PAT_TYPE_def,no_closures_def,PULL_EXISTS] >>
+  rw[] >>
+  TRY (
+    qmatch_assum_rename_tac`LIST_TYPE PATLANG_EXP_PAT_TYPE x1 y1`[] >>
+    rator_x_assum`LIST_TYPE`mp_tac >> last_x_assum mp_tac >>
+    rpt(pop_assum kall_tac) >>
+    map_every qid_spec_tac[`y1`,`x1`] >>
+    Induct >> simp[ml_repl_stepTheory.LIST_TYPE_def,no_closures_def,PULL_EXISTS] >>
+    rw[] >> METIS_TAC[] ) >>
+  METIS_TAC[EqualityType_thm,EqualityType_NUM,EqualityType_PATLANG_OP_PAT_TYPE,EqualityType_AST_LIT_TYPE])
+
+val PATLANG_EXP_PAT_TYPE_types_match = prove(
+  ``∀a b c d. PATLANG_EXP_PAT_TYPE a b ∧ PATLANG_EXP_PAT_TYPE c d ⇒ types_match b d``,
+  ho_match_mp_tac ml_repl_stepTheory.PATLANG_EXP_PAT_TYPE_ind >>
+  simp[ml_repl_stepTheory.PATLANG_EXP_PAT_TYPE_def,types_match_def,PULL_EXISTS] >> rw[] >>
+  Cases_on`c`>>fs[ml_repl_stepTheory.PATLANG_EXP_PAT_TYPE_def,types_match_def] >> rw[] >>
+  TRY (
+    qmatch_assum_rename_tac`LIST_TYPE PATLANG_EXP_PAT_TYPE x1 y1`[] >>
+    rator_x_assum`LIST_TYPE`mp_tac >>
+    qmatch_assum_rename_tac`LIST_TYPE PATLANG_EXP_PAT_TYPE x2 y2`[] >>
+    rator_x_assum`LIST_TYPE`mp_tac >>
+    last_x_assum mp_tac >>
+    rpt(pop_assum kall_tac) >>
+    map_every qid_spec_tac[`y2`,`y1`,`x1`,`x2`] >>
+    Induct >> simp[ml_repl_stepTheory.LIST_TYPE_def] >- (
+      Cases >> simp[ml_repl_stepTheory.LIST_TYPE_def,types_match_def,PULL_EXISTS] ) >>
+    gen_tac >> Cases >> simp[ml_repl_stepTheory.LIST_TYPE_def,PULL_EXISTS] >> rw[] >>
+    rw[types_match_def] >> METIS_TAC[] ) >>
+  METIS_TAC[EqualityType_thm,EqualityType_NUM,EqualityType_PATLANG_OP_PAT_TYPE,EqualityType_AST_LIT_TYPE])
+
+val PATLANG_EXP_PAT_TYPE_11 = prove(
+  ``∀a b c d. PATLANG_EXP_PAT_TYPE a b ∧ PATLANG_EXP_PAT_TYPE c d ⇒ (a = c ⇔ b = d)``,
+  ho_match_mp_tac ml_repl_stepTheory.PATLANG_EXP_PAT_TYPE_ind >>
+  simp[ml_repl_stepTheory.PATLANG_EXP_PAT_TYPE_def,PULL_EXISTS] >> rw[] >>
+  Cases_on`c`>>fs[ml_repl_stepTheory.PATLANG_EXP_PAT_TYPE_def] >> rw[] >>
+  TRY (
+    qmatch_assum_rename_tac`LIST_TYPE PATLANG_EXP_PAT_TYPE x1 y1`[] >>
+    rator_x_assum`LIST_TYPE`mp_tac >>
+    qmatch_assum_rename_tac`LIST_TYPE PATLANG_EXP_PAT_TYPE x2 y2`[] >>
+    rator_x_assum`LIST_TYPE`mp_tac >>
+    ((qmatch_assum_rename_tac`PATLANG_EXP_PAT_TYPE a1 b1`[] >>
+      rator_x_assum`PATLANG_EXP_PAT_TYPE`mp_tac >>
+      qmatch_assum_rename_tac`PATLANG_EXP_PAT_TYPE c1 d1`[] >>
+      strip_tac) ORELSE
+     (qmatch_assum_rename_tac`NUM a1 b1`[] >>
+      rator_x_assum`NUM`mp_tac >>
+      qmatch_assum_rename_tac`NUM c1 d1`[] >>
+      strip_tac) ORELSE
+     (qmatch_assum_rename_tac`PATLANG_OP_PAT_TYPE a1 b1`[] >>
+      rator_x_assum`PATLANG_OP_PAT_TYPE`mp_tac >>
+      qmatch_assum_rename_tac`PATLANG_OP_PAT_TYPE c1 d1`[] >>
+      strip_tac)) >>
+    `c1 = a1 ⇔ d1 = b1` by METIS_TAC[EqualityType_thm,EqualityType_PATLANG_OP_PAT_TYPE,EqualityType_NUM] >> simp[] >>
+    last_x_assum mp_tac >>
+    rpt(pop_assum kall_tac) >>
+    map_every qid_spec_tac[`y2`,`y1`,`x1`,`x2`] >>
+    Induct >> simp[ml_repl_stepTheory.LIST_TYPE_def] >- (
+      Cases >> simp[ml_repl_stepTheory.LIST_TYPE_def,PULL_EXISTS] ) >>
+    gen_tac >> Cases >> simp[ml_repl_stepTheory.LIST_TYPE_def,PULL_EXISTS] >> rw[] >>
+    rw[] >> METIS_TAC[] ) >>
+  METIS_TAC[EqualityType_thm,EqualityType_NUM,EqualityType_PATLANG_OP_PAT_TYPE,EqualityType_AST_LIT_TYPE])
+
+val EqualityType4 = prove(
+  ``EqualityType PATLANG_EXP_PAT_TYPE``,
+  METIS_TAC[EqualityType_thm,PATLANG_EXP_PAT_TYPE_no_closures,PATLANG_EXP_PAT_TYPE_types_match,PATLANG_EXP_PAT_TYPE_11])
+
+val AST_EXP_TYPE_no_closures = prove(
+  ``∀a b. AST_EXP_TYPE a b ⇒ no_closures b``,
+  ho_match_mp_tac ml_repl_stepTheory.AST_EXP_TYPE_ind >>
+  simp[ml_repl_stepTheory.AST_EXP_TYPE_def,PULL_EXISTS,no_closures_def] >> rw[] >>
+  TRY (
+    qmatch_assum_rename_tac`LIST_TYPE R x1 y1`["R"] >>
+    rator_x_assum`LIST_TYPE`mp_tac >>
+    last_x_assum mp_tac >>
+    rpt(pop_assum kall_tac) >>
+    map_every qid_spec_tac[`y1`,`x1`] >>
+    Induct >> simp[ml_repl_stepTheory.LIST_TYPE_def,PULL_EXISTS,no_closures_def] >>
+    qx_gen_tac`p` >> TRY(PairCases_on`p`) >>
+    simp[ml_repl_stepTheory.PAIR_TYPE_def,PULL_EXISTS,no_closures_def] >>
+    rw[] >>
+    METIS_TAC[EqualityType_thm,EqualityType_LIST_TYPE_CHAR,EqualityType3] ) >>
+  METIS_TAC[EqualityType_thm,EqualityType_OPTION_TYPE_LIST_TYPE_CHAR,
+            EqualityType_AST_LOP_TYPE,EqualityType_AST_OP_TYPE,
+            EqualityType_LIST_TYPE_CHAR,EqualityType_AST_ID_TYPE_LIST_TYPE_CHAR,
+            EqualityType_OPTION_TYPE_AST_ID_TYPE_LIST_TYPE_CHAR,
+            EqualityType_AST_LIT_TYPE])
+
+val AST_EXP_TYPE_types_match = prove(
+  ``∀a b c d. AST_EXP_TYPE a b ∧ AST_EXP_TYPE c d ⇒ types_match b d``,
+  ho_match_mp_tac ml_repl_stepTheory.AST_EXP_TYPE_ind >>
+  simp[ml_repl_stepTheory.AST_EXP_TYPE_def,PULL_EXISTS] >> rw[] >>
+  Cases_on`c`>>fs[ml_repl_stepTheory.AST_EXP_TYPE_def,types_match_def] >> rw[] >>
+  TRY (
+    qmatch_assum_rename_tac`LIST_TYPE R x1 y1`["R"] >>
+    rator_x_assum`LIST_TYPE`mp_tac >>
+    qmatch_assum_rename_tac`LIST_TYPE R x2 y2`["R"] >>
+    rator_x_assum`LIST_TYPE`mp_tac >>
+    last_x_assum mp_tac >>
+    rpt(pop_assum kall_tac) >>
+    map_every qid_spec_tac[`y1`,`x1`,`y2`,`x2`] >>
+    Induct >> simp[ml_repl_stepTheory.LIST_TYPE_def,PULL_EXISTS,types_match_def] >- (
+      Cases >> simp[ml_repl_stepTheory.LIST_TYPE_def,PULL_EXISTS,types_match_def] ) >>
+    qx_gen_tac`p` >> TRY(PairCases_on`p`) >>
+    simp[ml_repl_stepTheory.PAIR_TYPE_def,PULL_EXISTS] >>
+    gen_tac >> Cases >> simp[PULL_EXISTS,ml_repl_stepTheory.LIST_TYPE_def] >>
+    TRY(PairCases_on`h`)>>simp[ml_repl_stepTheory.PAIR_TYPE_def,PULL_EXISTS] >>
+    rw[types_match_def] >>
+    fs[FORALL_PROD] >>
+    PROVE_TAC[EqualityType_thm,EqualityType_LIST_TYPE_CHAR,EqualityType3] ) >>
+  METIS_TAC[EqualityType_thm,EqualityType_OPTION_TYPE_LIST_TYPE_CHAR,
+            EqualityType_AST_LOP_TYPE,EqualityType_AST_OP_TYPE,
+            EqualityType_LIST_TYPE_CHAR,EqualityType_AST_ID_TYPE_LIST_TYPE_CHAR,
+            EqualityType_OPTION_TYPE_AST_ID_TYPE_LIST_TYPE_CHAR,
+            EqualityType_AST_LIT_TYPE])
+
+val AST_EXP_TYPE_11 = prove(
+  ``∀a b c d. AST_EXP_TYPE a b ∧ AST_EXP_TYPE c d ⇒ (a = c ⇔ b = d)``,
+  ho_match_mp_tac ml_repl_stepTheory.AST_EXP_TYPE_ind >>
+  simp[ml_repl_stepTheory.AST_EXP_TYPE_def,PULL_EXISTS] >> rw[] >>
+  Cases_on`c`>>fs[ml_repl_stepTheory.AST_EXP_TYPE_def] >> rw[] >>
+  TRY (
+    qmatch_assum_rename_tac`LIST_TYPE R x1 y1`["R"] >>
+    rator_x_assum`LIST_TYPE`mp_tac >>
+    qmatch_assum_rename_tac`LIST_TYPE R x2 y2`["R"] >>
+    rator_x_assum`LIST_TYPE`mp_tac >>
+    REWRITE_TAC[AND_IMP_INTRO] >>
+    last_x_assum mp_tac >>
+    MATCH_MP_TAC SWAP_IMP >>
+    REWRITE_TAC[GSYM AND_IMP_INTRO] >>
+    TRY(
+      qmatch_assum_rename_tac`R a1 b1`["R"] >>
+      qpat_assum`R a1 b1`mp_tac >>
+      qmatch_assum_rename_tac`R a2 b2`["R"] >>
+      strip_tac >>
+      `a2 = a1 ⇔ b2 = b1` by
+        METIS_TAC[EqualityType_thm,EqualityType_AST_OP_TYPE,
+                  EqualityType_OPTION_TYPE_AST_ID_TYPE_LIST_TYPE_CHAR] >>
+      simp[] ) >>
+    rpt(pop_assum kall_tac) >>
+    map_every qid_spec_tac[`y1`,`x1`,`y2`,`x2`] >>
+    Induct >> simp[ml_repl_stepTheory.LIST_TYPE_def,PULL_EXISTS] >- (
+      Cases >> simp[ml_repl_stepTheory.LIST_TYPE_def,PULL_EXISTS] ) >>
+    qx_gen_tac`p` >> TRY(PairCases_on`p`) >>
+    simp[ml_repl_stepTheory.PAIR_TYPE_def,PULL_EXISTS] >>
+    Cases >> simp[PULL_EXISTS,ml_repl_stepTheory.LIST_TYPE_def] >>
+    TRY(PairCases_on`h`)>>simp[ml_repl_stepTheory.PAIR_TYPE_def,PULL_EXISTS] >>
+    rw[] >> fs[FORALL_PROD] >>
+    first_x_assum(fn th => first_x_assum(mp_tac o MATCH_MP th)) >>
+    disch_then(fn th => first_x_assum(mp_tac o MATCH_MP th)) >>
+    TRY(discharge_hyps >- metis_tac[]) >>
+    metis_tac[EqualityType_thm,EqualityType_LIST_TYPE_CHAR,EqualityType3] ) >>
+  METIS_TAC[EqualityType_thm,EqualityType_OPTION_TYPE_LIST_TYPE_CHAR,
+            EqualityType_AST_LOP_TYPE,EqualityType_AST_OP_TYPE,
+            EqualityType_LIST_TYPE_CHAR,EqualityType_AST_ID_TYPE_LIST_TYPE_CHAR,
+            EqualityType_OPTION_TYPE_AST_ID_TYPE_LIST_TYPE_CHAR,
+            EqualityType_AST_LIT_TYPE])
+
+val EqualityType5 = prove(
+  ``EqualityType AST_EXP_TYPE``,
+  METIS_TAC[EqualityType_thm,AST_EXP_TYPE_no_closures,AST_EXP_TYPE_types_match,AST_EXP_TYPE_11])
+
+val INFER_T_INFER_T_TYPE_no_closures = prove(
+  ``∀a b. INFER_T_INFER_T_TYPE a b ⇒ no_closures b``,
+  ho_match_mp_tac ml_repl_stepTheory.INFER_T_INFER_T_TYPE_ind >>
+  simp[ml_repl_stepTheory.INFER_T_INFER_T_TYPE_def,no_closures_def,PULL_EXISTS] >> rw[] >>
+  TRY (
+    qmatch_assum_rename_tac`LIST_TYPE R a b`["R"] >>
+    rator_x_assum`LIST_TYPE`mp_tac >>
+    last_x_assum mp_tac >>
+    map_every qid_spec_tac[`b`,`a`] >>
+    rpt(pop_assum kall_tac) >>
+    Induct >> simp[ml_repl_stepTheory.LIST_TYPE_def,PULL_EXISTS,no_closures_def] >>
+    rw[] >> METIS_TAC[]) >>
+  METIS_TAC[EqualityType_thm,EqualityType_NUM,EqualityType_AST_TCTOR_TYPE])
+
+val INFER_T_INFER_T_TYPE_types_match = prove(
+  ``∀a b c d. INFER_T_INFER_T_TYPE a b ∧ INFER_T_INFER_T_TYPE c d ⇒ types_match b d``,
+  ho_match_mp_tac ml_repl_stepTheory.INFER_T_INFER_T_TYPE_ind >>
+  simp[ml_repl_stepTheory.INFER_T_INFER_T_TYPE_def,PULL_EXISTS] >> rw[] >>
+  Cases_on`c`>>fs[ml_repl_stepTheory.INFER_T_INFER_T_TYPE_def] >> rw[types_match_def] >>
+  TRY (
+    qmatch_assum_rename_tac`LIST_TYPE R a b`["R"] >>
+    rator_x_assum`LIST_TYPE`mp_tac >>
+    qmatch_assum_rename_tac`LIST_TYPE R c d`["R"] >>
+    rator_x_assum`LIST_TYPE`mp_tac >>
+    last_x_assum mp_tac >>
+    map_every qid_spec_tac[`b`,`a`,`d`,`c`] >>
+    rpt(pop_assum kall_tac) >>
+    Induct >> simp[ml_repl_stepTheory.LIST_TYPE_def,PULL_EXISTS] >> rw[] >>
+    Cases_on`a`>>fs[ml_repl_stepTheory.LIST_TYPE_def] >>
+    rw[types_match_def] >> METIS_TAC[]) >>
+  METIS_TAC[EqualityType_thm,EqualityType_NUM,EqualityType_AST_TCTOR_TYPE])
+
+val INFER_T_INFER_T_TYPE_11 = prove(
+  ``∀a b c d. INFER_T_INFER_T_TYPE a b ∧ INFER_T_INFER_T_TYPE c d ⇒ (a = c ⇔ b = d)``,
+  ho_match_mp_tac ml_repl_stepTheory.INFER_T_INFER_T_TYPE_ind >>
+  simp[ml_repl_stepTheory.INFER_T_INFER_T_TYPE_def,PULL_EXISTS] >> rw[] >>
+  Cases_on`c`>>fs[ml_repl_stepTheory.INFER_T_INFER_T_TYPE_def] >> rw[] >>
+  TRY (
+    qmatch_assum_rename_tac`LIST_TYPE R a b`["R"] >>
+    rator_x_assum`LIST_TYPE`mp_tac >>
+    qmatch_assum_rename_tac`LIST_TYPE R c d`["R"] >>
+    rator_x_assum`LIST_TYPE`mp_tac >>
+    last_x_assum mp_tac >>
+    qmatch_assum_rename_tac`R u v`["R"] >> pop_assum mp_tac >>
+    qmatch_assum_rename_tac`R w x`["R"] >> strip_tac >>
+    `w = u ⇔ x = v` by METIS_TAC[EqualityType_thm,EqualityType_AST_TCTOR_TYPE] >> simp[] >>
+    map_every qid_spec_tac[`b`,`a`,`d`,`c`] >>
+    rpt(pop_assum kall_tac) >>
+    Induct >> simp[ml_repl_stepTheory.LIST_TYPE_def,PULL_EXISTS] >> rw[] >>
+    Cases_on`a`>>fs[ml_repl_stepTheory.LIST_TYPE_def] >>
+    rw[types_match_def] >> METIS_TAC[]) >>
+  METIS_TAC[EqualityType_thm,EqualityType_NUM,EqualityType_AST_TCTOR_TYPE])
+
+val EqualityType6 = prove(
+  ``EqualityType INFER_T_INFER_T_TYPE``,
+  METIS_TAC[EqualityType_thm,INFER_T_INFER_T_TYPE_no_closures,INFER_T_INFER_T_TYPE_types_match,INFER_T_INFER_T_TYPE_11])
+
+val EqualityTypes = [EqualityType1, EqualityType2, EqualityType3, EqualityType4, EqualityType5, EqualityType6]
+
+val evaluate_repl_decs = DISCH_ALL module_thm |> REWRITE_RULE EqualityTypes
+
+val INPUT_TYPE_def = Define `
+  INPUT_TYPE =
+  ^(find_term (can (match_term ``OPTION_TYPE xx``)) (concl evaluate_repl_decs))`;
+
+val OUTPUT_TYPE_def = Define `
+  OUTPUT_TYPE =
+  ^(find_term (can (match_term ``SUM_TYPE xx yy``)) (concl evaluate_repl_decs))`;
+
+val OPTION_TYPE_no_closures = prove(
+  ``(∀a b. A a b ⇒ no_closures b) ⇒ ∀a b. OPTION_TYPE A a b ⇒ no_closures b``,
+  strip_tac >> Cases >> simp[ml_repl_stepTheory.OPTION_TYPE_def,no_closures_def,PULL_EXISTS] >> METIS_TAC[])
+
+val PAIR_TYPE_no_closures = prove(
+  ``(∀a b. A a b ⇒ no_closures b) ∧ (∀a b. B a b ⇒ no_closures b) ⇒ ∀a b. PAIR_TYPE A B a b ⇒ no_closures b``,
+  strip_tac >> Cases >> simp[ml_repl_stepTheory.PAIR_TYPE_def,no_closures_def,PULL_EXISTS] >> METIS_TAC[])
+
+val LIST_TYPE_no_closures = prove(
+  ``(∀a b. A a b ⇒ no_closures b) ⇒ ∀a b. LIST_TYPE A a b ⇒ no_closures b``,
+  strip_tac >> Induct >> simp[ml_repl_stepTheory.LIST_TYPE_def,no_closures_def,PULL_EXISTS] >>
+  METIS_TAC[] )
+
+val FMAP_TYPE_no_closures = prove(
+  ``(∀a b. A a b ⇒ no_closures b) ∧ (∀a b. B a b ⇒ no_closures b) ⇒ ∀a b. FMAP_TYPE A B a b ⇒ no_closures b``,
+  strip_tac >>
+  Induct >> simp[ml_repl_stepTheory.FMAP_TYPE_def,PULL_EXISTS] >> rw[] >>
+  METIS_TAC[LIST_TYPE_no_closures,PAIR_TYPE_no_closures])
+
+val COMPILER_COMPILER_STATE_TYPE_no_closures = prove(
+  ``∀a b. COMPILER_COMPILER_STATE_TYPE a b ⇒ no_closures b``,
+  Cases >>
+  simp[ml_repl_stepTheory.COMPILER_COMPILER_STATE_TYPE_def,PULL_EXISTS,no_closures_def] >>
+  rw[] >>
+  rpt (
+    qmatch_rename_tac`ml_translator$no_closures z`[] >>
+    qmatch_assum_abbrev_tac`A a z` >>
+    qpat_assum`A a z`mp_tac >>
+    unabbrev_all_tac >>
+    (( match_mp_tac PAIR_TYPE_no_closures ) ORELSE
+     ( match_mp_tac FMAP_TYPE_no_closures ) ORELSE
+     ( match_mp_tac OPTION_TYPE_no_closures )
+    ) >> rw[]) >>
+  METIS_TAC[EqualityType_thm,EqualityType_NUM,EqualityType_LIST_TYPE_CHAR,
+            EqualityType_SEMANTICPRIMITIVES_TID_OR_EXN_TYPE,
+            EqualityType_AST_ID_TYPE_LIST_TYPE_CHAR,
+            EqualityType_SPTREE_SPT_TYPE_UNIT_TYPE])
+
+val LIST_TYPE_CHAR_no_closures =
+  EqualityType_LIST_TYPE_CHAR |> REWRITE_RULE[EqualityType_thm] |> CONJUNCT1
+
+val REPL_FUN_REPL_FUN_STATE_TYPE_no_closures = prove(
+  ``∀a b. REPL_FUN_REPL_FUN_STATE_TYPE a b ⇒ no_closures b``,
+  Cases >>
+  simp[ml_repl_stepTheory.REPL_FUN_REPL_FUN_STATE_TYPE_def,PULL_EXISTS,no_closures_def] >>
+  rw[] >>
+  rpt (
+    qmatch_rename_tac`ml_translator$no_closures z`[] >>
+    qmatch_assum_abbrev_tac`A a z` >>
+    qpat_assum`A a z`mp_tac >>
+    unabbrev_all_tac >>
+    (( match_mp_tac PAIR_TYPE_no_closures ) ORELSE
+     ( match_mp_tac FMAP_TYPE_no_closures ) ORELSE
+     ( MATCH_ACCEPT_TAC LIST_TYPE_CHAR_no_closures) ORELSE
+     ( match_mp_tac LIST_TYPE_no_closures ) ORELSE
+     ( match_mp_tac OPTION_TYPE_no_closures ) ORELSE
+     ( MATCH_ACCEPT_TAC COMPILER_COMPILER_STATE_TYPE_no_closures )
+    ) >> rw[]) >>
+  METIS_TAC[EqualityType_thm,EqualityType_NUM,
+            EqualityType_AST_ID_TYPE_LIST_TYPE_CHAR,
+            EqualityType2, EqualityType6,
+            EqualityType_SEMANTICPRIMITIVES_TID_OR_EXN_TYPE])
+
+val INPUT_TYPE_no_closures = store_thm("INPUT_TYPE_no_closures",
+  ``∀a b. INPUT_TYPE a b ⇒ no_closures b``,
+  simp[INPUT_TYPE_def] >>
+  match_mp_tac OPTION_TYPE_no_closures >>
+  match_mp_tac PAIR_TYPE_no_closures >>
+  conj_tac >- (
+    METIS_TAC[
+      EqualityType_LIST_TYPE,
+      EqualityType_thm,
+      find_equality_type_thm``LEXER_FUN_SYMBOL_TYPE``,
+      EqualityType_LIST_TYPE_CHAR,
+      EqualityType_INT] ) >>
+  match_mp_tac PAIR_TYPE_no_closures >>
+  conj_tac >- ( METIS_TAC[EqualityType_thm, EqualityType_BOOL] ) >>
+  match_mp_tac PAIR_TYPE_no_closures >>
+  conj_tac >- (
+    match_mp_tac PAIR_TYPE_no_closures >>
+    conj_tac >- ( METIS_TAC[EqualityType_thm, EqualityType_NUM] ) >>
+    match_mp_tac FMAP_TYPE_no_closures >>
+    METIS_TAC[EqualityType_thm, EqualityType_NUM] ) >>
+  match_mp_tac PAIR_TYPE_no_closures >>
+  reverse conj_asm1_tac >- (pop_assum ACCEPT_TAC) >>
+  MATCH_ACCEPT_TAC REPL_FUN_REPL_FUN_STATE_TYPE_no_closures)
+
+val _ = save_thm("evaluate_repl_decs",evaluate_repl_decs
+  |> REWRITE_RULE [GSYM INPUT_TYPE_def, GSYM OUTPUT_TYPE_def])
 
 val _ = Theory.delete_binding "side_translator_state_thm";
 
